



Let  $G = M \otimes I + I \otimes M - C \cdot \left(\frac{1}{2N_z}\right)$

↑ Kronecker

the matrix  
 $C_{zz,zz} = \frac{1}{2N_z}$   
 $= 0$  otherwise

num  $\begin{cases} M_{xy} = \text{rate of linear migr from } x \text{ to } y, x \neq y \\ M_{xx} = -\sum_{y \neq x} M_{xy} \end{cases}$

$$A \otimes B = \begin{bmatrix} A_{11}B & A_{12}B & A_{13}B \\ \vdots & \vdots & \vdots \\ \vdots & \vdots & A_{33}B \end{bmatrix}$$

$$G_{xy,uv} = \begin{cases} M_{xu} & \text{if } y=v \\ M_{yv} & \text{if } x=u \\ -\sum_z M_{xz} - \sum_z M_{yz} & \text{if } x=y, y=v, x \neq y \\ \text{(Same)} -\frac{1}{2N_z} & \text{if } x=u=y=v \\ 0 & \text{otherwise} \end{cases}$$

$$e^{tG} = \sum_{n=0}^{\infty} \frac{t^n G^n}{n!}$$

goal: Coal rate for locs started at  $(x, y)$  at time  $t$  ago

$$r_{xy}(t) = \sum_{z \text{ locs}} \mathbb{P}[\text{both } X_t = Y_t = z] \cdot \frac{1}{2N_z}$$

↑ Kronecker

$$\mathbb{P}\{X_t = u, Y_t = v \mid X_0 = x, Y_0 = y\} = (e^{tG})_{xy,uv}$$

Let  $f_{xy}(t) = \mathbb{P}\{\text{haven't yet coal-seed} \mid X_0 = x, Y_0 = y\}$

$$= \sum_{uv} (e^{tG})_{xy,uv}$$

$$r_{xy}(t) = \sum_z (e^{tG})_{xy,zz} \cdot \frac{1}{2N_z}$$